old/PushRelabel.dfy
@@ -1,0 +1,205 @@
+include "Graph.dfy"
+include "Flow.dfy"
+
+module Algorithm {
+  import Graph
+  import FlowGraph
+
+  class PushRelabel {
+    const V: nat
+    const s: nat
+    const t: nat
+    const capacity: array2<nat>
+
+    var flow: array2<int>
+    var height: array<nat>
+    var excess: array<int>
+
+    var buckets: array<set<nat>>
+    var max_height: int
+
+    predicate ValidBucketsStructure()
+      reads this
+    {
+      buckets.Length == 2 * V
+    }
+
+    predicate ValidBuckets()
+      reads this, height, excess, buckets
+      requires FlowGraph.ValidHeightShape(V, height)
+      requires FlowGraph.ValidExcessShape(V, excess)
+      requires ValidBucketsStructure()
+    {
+      -1 <= max_height < 2 * V &&
+      // max_height is the upper bound
+      (forall v :: (0 <= v < V && v!= s && v != t && excess[v] > 0) ==> height[v] <= max_height) &&
+      // If a non terminal node is active it must be in the bucket of its current height
+      (forall v :: (0 <= v < V && v != s && v != t && excess[v] > 0) ==> v in buckets[height[v]]) &&
+      // If a node is in a bucket it must be active and cannot be a terminal node
+      (forall h, v :: (0 <= h < 2 * V && 0 <= v < V && v in buckets[h]) ==> (excess[v] > 0 && v != s && v != t)) &&
+      // If a node is in a bucket it must have the height of that bucket
+      (forall h, v :: (0 <= h < 2 * V && 0 <= v < V && v in buckets[h]) ==> height[v] == h)
+    }
+
+    predicate ValidStructure()
+      reads this
+    {
+      Graph.ValidGraph(V, s, t) &&
+      FlowGraph.ValidFlowMatrixShape(V, flow) &&
+      FlowGraph.ValidCapacityMatrixShape(V, capacity) &&
+      FlowGraph.ValidHeightShape(V, height) &&
+      FlowGraph.ValidExcessShape(V, excess) &&
+      ValidBucketsStructure()
+    }
+
+    predicate Valid()
+      reads this, capacity, flow, height, excess, buckets
+    {
+      ValidStructure() &&
+      FlowGraph.ValidPreflow(V, s, t, capacity, flow) &&
+      FlowGraph.ValidExcess(V, s, t, capacity, flow, excess) &&
+      FlowGraph.ValidLabeling(V, s, t, capacity, flow, height) &&
+      ValidBuckets()
+    }
+
+    function ResidualCapacity(v: nat, w: nat): nat
+      reads this, capacity, flow
+      requires Graph.ValidGraph(V, s, t)
+      requires FlowGraph.ValidFlowMatrixShape(V, flow)
+      requires FlowGraph.ValidCapacityMatrixShape(V, capacity)
+      requires FlowGraph.ValidPreflow(V, s, t, capacity, flow)
+      requires Graph.ValidNode(V, v) && Graph.ValidNode(V, w)
+    {
+      FlowGraph.ResidualCapacity(V, s, t, capacity, flow, v, w)
+    }
+
+    method Push(v: nat, w: nat)
+      requires Valid()
+
+      // Preconditions for a valid push:
+      requires Graph.ValidNode(V, v) && Graph.ValidNode(V, w)   // v and w must be nodes in the Graph
+      requires !FlowGraph.NodeIsSourceOrSink(v, s, t)           // v cannot be equal to the source or sink
+      requires FlowGraph.NodeIsActive(V, v, excess)             // w must be active
+      requires ResidualCapacity(v, w) > 0                       // There must be pipe space
+      requires height[v] == height[w] + 1                       // Water must flow exactly one step downhill
+
+      // postconditions
+      ensures Valid()
+
+      modifies flow, excess, buckets
+    {
+      // Calculate how much water we can push
+      var delta := excess[v];
+      var res_cap := ResidualCapacity(v, w);
+      if (res_cap < delta) {
+        delta := res_cap;
+      }
+
+      label BeforeMutation:
+      flow[v, w] := flow[v, w] + delta;
+      flow[w, v] := flow[w, v] - delta;
+      FlowGraph.LemmaFlowSumAfterPush@BeforeMutation(V, flow, v, w, delta, V);
+
+      // Store w's inital active state far later use
+      var old_w_active := FlowGraph.NodeIsActive(V, w, excess);
+
+      excess[v] := excess[v] - delta;
+      excess[w] := excess[w] + delta;
+
+      if (excess[v] == 0) {
+        buckets[height[v]] := buckets[height[v]] - {v};
+      }
+
+      // Update the Highest-Label Buckets
+      // If w was NOT active and w is not s or t, which implies it is active now, it enters the buckets.
+      if (!old_w_active && !FlowGraph.NodeIsSourceOrSink(w, s, t)) {
+        assert FlowGraph.NodeIsActive(V, w, excess);
+
+        buckets[height[w]] := buckets[height[w]] + {w};
+        // We don't need to update max_height here because water flows downhill
+        // height[w] is strictly less than height[v], so it cannot become the new max_height.
+      }
+    }
+
+    method Relabel(v: nat)
+      requires Valid()
+
+      // Preconditions for a valid relabel:
+      requires Graph.ValidNode(V, v)                  // v must be a node in the Graph
+      requires !FlowGraph.NodeIsSourceOrSink(v, s, t) // v cannot be equal to the source or sink
+      requires FlowGraph.NodeIsActive(V, v, excess)   // v must be active
+      // v cannot be relabeled if it has a downhill neighbor
+      requires forall w :: 0 <= w < V && ResidualCapacity(v, w) > 0 ==> height[v] <= height[w]
+
+      // Postconditions
+      ensures Valid()
+
+      modifies this, height, buckets
+    {
+      // Find the lowest neighbor in the residual graph
+      // We initialize minHeightNeighbour to an impossibly high value (2 * V)
+      var minHeightNeighbour: nat := 2 * V;
+      var w := 0;
+      while (w < V)
+        invariant 0 <= w <= V
+        invariant minHeightNeighbour <= 2 * V
+        invariant forall k :: 0 <= k < w && ResidualCapacity(v, k) > 0 ==> minHeightNeighbour <= height[k]
+
+        // Because v had no downhill neighbors, height[v] MUST be <= minHeightNeighbour.
+        // invariant so that Dafny does not forget
+        invariant height[v] <= minHeightNeighbour
+      {
+        if (ResidualCapacity(v, w) > 0) {
+          if (height[w] < minHeightNeighbour) {
+            minHeightNeighbour := height[w];
+          }
+        }
+        w := w + 1;
+      }
+      // Assert minHeightNeighbour is actual minimum
+      assert forall k :: 0 <= k < V && ResidualCapacity(v, k) > 0 ==> minHeightNeighbour <= height[k];
+
+      // ------ Lemma's and proofs needed to prove height[v] < 2 * V after relabel ------
+      // Prove a path to source exists from v
+      FlowGraph.Lemma_ActiveVertexHasPathToSource(V, s, t, capacity, flow, excess, v);
+      // Extract that path
+      ghost var pathToSource :| FlowGraph.IsSimpleResidualPath(V, s, t, capacity, flow, pathToSource) && pathToSource[0] == v && pathToSource[|pathToSource|-1] == s;
+
+      // Since v != s, the path has at least 2 nodes. Grab the next node in the path
+      assert |pathToSource| >= 2;
+      ghost var pathToSourceNextNode := pathToSource[1];
+
+      // Because v and pathToSourceNextNode are connected on a residual path, there is residual capacity
+      assert FlowGraph.ResidualCapacity(V, s, t, capacity, flow, v, pathToSourceNextNode) > 0;
+
+      // get the remainder of the path (from pathToSourceNextNode to s)
+      ghost var pathToSourceWithoutV := pathToSource[1..];
+
+      // Apply length and telescoping height lemmas
+      Graph.Lemma_SimplePathHasBoundedLength(V, pathToSource);
+      assert |pathToSource| <= V;
+      FlowGraph.Lemma_PathTelescopingHeight(V, s, t, capacity, flow, height, pathToSourceWithoutV);
+      assert height[pathToSourceNextNode] <= height[s] + |pathToSourceWithoutV| - 1;
+      assert height[pathToSourceNextNode] <= V + (V - 1) - 1; // Since height[s] == V && ((|pathToSource| <= V) ==> (|pathToSourceWithoutV| <= V - 1))
+      assert height[pathToSourceNextNode] <= 2 * V - 2;
+      assert height[pathToSourceNextNode] < 2 * V - 1;
+
+      // This proves there exists a path to source where height[pathToSourceNextNode] < 2 * V - 1
+      // minHeightNeighbour is the neighbour on the path where the next node has the minimum height
+      // this means the following assertions also holds
+      assert minHeightNeighbour < 2 * V - 1;
+      assert minHeightNeighbour + 1 < 2 * V;
+      // ------------
+
+      buckets[height[v]] := buckets[height[v]] - {v};
+
+      height[v] := minHeightNeighbour + 1;
+
+      buckets[height[v]] := buckets[height[v]] + {v};
+
+      if (height[v] > max_height) {
+        max_height := height[v];
+      }
+    }
+  }
+}
